src/JSON/JSON.AST.dfy
@@ -1,0 +1,11 @@
+module {:options "-functionSyntax:4"} JSON.AST {
+  datatype KV = KV(k: string, v: Value)
+  datatype Decimal = Decimal(n: int, e10: nat) // (n) * 10^(e10)
+  datatype Value =
+    | Null
+    | Bool(b: bool)
+    | String(str: string)
+    | Number(num: Decimal)
+    | Object(obj: seq<KV>) // Not a map to preserve order
+    | Array(arr: seq<Value>)
+}
