src/JSON/Str.dfy
@@ -1,0 +1,88 @@
+include "../BoundedInts.dfy"
+
+module {:options "-functionSyntax:4"} Str {
+  module Private {
+    function Digits(n: int, base: int): (digits: seq<int>)
+      requires base > 1
+      requires n >= 0
+      decreases n
+      ensures forall d | d in digits :: 0 <= d < base
+    {
+      if n == 0 then
+        []
+      else
+        assert n > 0;
+        assert base > 1;
+        assert n < base * n;
+        assert n / base < n;
+        Digits(n / base, base) + [n % base]
+    }
+
+    function OfDigits(digits: seq<int>, chars: seq<char>) : string
+      requires forall d | d in digits :: 0 <= d < |chars|
+    {
+      if digits == [] then ""
+      else
+        assert digits[0] in digits;
+        assert forall d | d in digits[1..] :: d in digits;
+        [chars[digits[0]]] + OfDigits(digits[1..], chars)
+    }
+  }
+
+  function OfInt_any(n: int, chars: seq<char>) : string
+    requires |chars| > 1
+  {
+    var base := |chars|;
+    if n == 0 then
+      "0"
+    else if n > 0 then
+      Private.OfDigits(Private.Digits(n, base), chars)
+    else
+      "-" + Private.OfDigits(Private.Digits(-n, base), chars)
+  }
+
+  const HEX_DIGITS := [
+    '0', '1', '2', '3', '4', '5', '6', '7', '8', '9',
+    'A', 'B', 'C', 'D', 'E', 'F']
+
+  function OfInt(n: int, base: int := 10) : string
+    requires 2 <= base <= 16
+  {
+    OfInt_any(n, HEX_DIGITS[..base])
+  }
+
+  method Test() { // FIXME {:test}?
+    expect OfInt(0, 10) == "0";
+    expect OfInt(3, 10) == "3";
+    expect OfInt(302, 10) == "302";
+    expect OfInt(-3, 10) == "-3";
+    expect OfInt(-302, 10) == "-302";
+  }
+
+  function OfBool(b: bool) : string {
+    if b then "true" else "false"
+  }
+
+  function OfChar(c: char) : string {
+    [c]
+  }
+
+  function Join(sep: string, strs: seq<string>) : string {
+    if |strs| == 0 then ""
+    else if |strs| == 1 then strs[0]
+    else strs[0] + sep + Join(sep, strs[1..])
+  }
+
+  function Concat(strs: seq<string>) : string {
+    Join("", strs)
+  }
+
+  import opened BoundedInts
+
+  function ToBytes(s: string) : seq<uint8>
+    requires forall c: char | c in s :: c as int < 256
+  {
+    seq(|s|, i requires 0 <= i < |s| =>
+      assert s[i] in s; s[i] as byte)
+  }
+}
